Dafny/LLVM/memory.i.dfy
@@ -18,46 +18,6 @@ type Block = seq<MemCell>
 type MemMap = map<nat, Block>
 datatype MemState = MemState(mem:MemMap, nextBlock:nat)
 
-
-// On initialization, the memory state is empty and contains no blocks
-predicate MemInit(s:MemState) {
-    && |s.mem| == 0
-    && s.nextBlock == 0
-}
-
-// Need to check every step to make sure memory is still valid
-predicate MemValid(s:MemState) {
-    && (forall bid | bid in s.mem :: bid < s.nextBlock)
-    && (forall bid | bid in s.mem :: BlockValid(s.mem[bid]))
-}
-
-
-datatype MemStep = 
-    | allocStep(bid:nat, size:nat)
-    | freeStep(bid:nat)
-    | storeStep(bid:nat, offset:nat, data:Data, n:bitWidth)
-    | stutterStep()
-
-predicate NextMemStep(s:MemState, s':MemState, step:MemStep)
-{
-    match step  
-        case allocStep(bid,size) => Alloc(s,s',bid,size)
-        case freeStep(bid) => Free(s,s',bid)
-        case storeStep(bid,offset,data,n) => (&& IsValidPtr(s, bid, offset,n)
-                                            && data.Int? && IntType(1, false) == data.itype
-                                            && (|s.mem[bid]| == 1 && Store(s,s',bid,offset,data)))
-        case stutterStep() => s == s'
-}
-
-// Describes valid Mem state transition 
-predicate MemStateNext(s:MemState,s':MemState,step:MemStep)
-{
-    MemValid(s)
-    && MemValid(s')
-    && NextMemStep(s,s',step)
-}
-
-
 // A newly-initialized block should start out uninitialized, meaning all its
 // members are muninit
 predicate IsUninit(b:Block) {
@@ -87,7 +47,12 @@ predicate IsValidPtr(s:MemState, bid:nat, offset:nat, size:bitWidth) {
     && bid in s.mem
     && offset < |s.mem[bid]|
     && validBitWidth(size)
-    && |s.mem[bid]| == size
+}
+
+// On initialization, the memory state is empty and contains no blocks
+predicate MemInit(s:MemState) {
+    && |s.mem| == 0
+    && s.nextBlock == 0
 }
 
 // A byte-memory cell is valid within a block if the surrounding memory cells starting
@@ -110,19 +75,38 @@ predicate BlockValid(b:Block) {
     forall offset | 0 < offset < |b| :: (b[offset].mb? ==> (b[offset].size > 0 && ByteMemValid(b, offset)))
 }
 
+// Need to check every step to make sure memory is still valid
+predicate MemValid(s:MemState) {
+    && (forall bid | bid in s.mem :: bid < s.nextBlock)
+    && (forall bid | bid in s.mem :: BlockValid(s.mem[bid]))
+}
 
+datatype MemStep = 
+    | allocStep(bid:nat, size:nat)
+    | freeStep(bid:nat)
+    | storeStep(bid:nat, offset:nat, data:Data, n:bitWidth)
+    | memCpyStep(bid:nat,bid':nat)
+    | stutterStep()
 
-// predicate MemStateNext(s:MemState,s':MemState)
-// {
-//     MemValid(s)
-//     && MemValid(s')
-//     && ( || s == s'
-//          || exists b,n :: Alloc(s,s',b,n)
-//          || exists b :: Free(s,s',b)
-//          || exists b:nat,o:nat,d:Data,n:bitWidth :: && IsValidPtr(s, b, o,n)
-//                                                     && d.Int? && IntType(1, false) == d.itype
-//                                                     && (|s.mem[b]| == 1 && Store(s,s',b,o,d)))
-// }
+predicate NextMemStep(s:MemState, s':MemState, step:MemStep)
+{
+    match step  
+        case allocStep(bid,size) => Alloc(s,s',bid,size)
+        case freeStep(bid) => Free(s,s',bid)
+        case storeStep(bid,offset,data,n) => (&& IsValidPtr(s, bid, offset,n)
+                                            && data.Int? && IntType(1, false) == data.itype
+                                            && (Store(s,s',bid,offset,data)))
+        case memCpyStep(bid,bid') => bid' in s'.mem && bid in s.mem && s'.mem[bid'] == s.mem[bid]
+        case stutterStep() => s == s'
+}
+
+// Describes valid Mem state transition 
+predicate MemStateNext(s:MemState,s':MemState,step:MemStep)
+{
+    MemValid(s)
+    && MemValid(s')
+    && NextMemStep(s,s',step)
+}
 // When a new block is allocated, all the previous blocks should remain the same,
 // and an unininitialized block of the appropriate size should be added with block
 // nextBlock
@@ -161,36 +145,18 @@ predicate Store(s:MemState, s':MemState, bid:nat, offset:nat, data:Data)
 {
     && s'.nextBlock == s.nextBlock
     && s'.mem == s.mem[bid := s.mem[bid][offset := mb(data.itype.size, DataToUInt8(data))]]
+    // && NextMemStep(s,s',MemStep.storeStep(bid,offset,data,1))
 }
-
-function evalALLOCA(s:MemState, size:nat): (out:Data)
-    requires MemValid(s)
-    // requires Alloc(s,s',s.nextBlock,size);
-    requires validBitWidth(size);
-     ensures out.Ptr?;
+lemma StoreImpliesStoreStep(s:MemState, s':MemState, bid:nat, offset:nat, data:Data)
+    requires IsValidPtr(s, bid, offset,1)
+    requires data.Int? && IntType(1, false) == data.itype;
+    requires Store(s,s',bid,offset,data);
 {
-    // && bid == s.nextBlock
-    // && s'.nextBlock == s.nextBlock + 1
-    // && s'.mem == s.mem[s.nextBlock := UninitBlock(size)]
-    var bid := s.nextBlock;
-    // assert Alloc(s,s',bid,size);
-    var d := (Ptr(bid,bid,0,size));
-    d
+    assert IsValidPtr(s, bid, offset,1);
+    assert data.Int? && IntType(1, false) == data.itype;
+    assert (Store(s,s',bid,offset,data));
+    assert NextMemStep(s, s', MemStep.storeStep(bid,offset,data,1));
 }
-
-function AllocaStep(s:MemState, size:nat): (out:MemState)
-    requires MemValid(s);
-    ensures MemValid(out);
-{
-    // s'.nextBlock := s.nextBlock + 1;
-     var x := s.mem[s.nextBlock := UninitBlock(size)];
-     var y:MemState := MemState(x,s.nextBlock + 1);
-     assert Alloc(s,y,s.nextBlock,size);
-     assert BlockValid(y.mem[s.nextBlock]);
-     assert MemValid(y);
-     y
-}
-
 // // Memory Access and Addressing Operations // 
 function evalLOAD(s:MemState,s':MemState,t:bitWidth,op1:Data): (out:Data)
     requires MemValid(s)
@@ -215,7 +181,6 @@ function evalGETELEMENTPTR(s:MemState,t:bitWidth,op1:Data,op2:Data): (out:Data)
     requires op1.Ptr? //TODO: Also could be vector of Ptrs
     requires validBitWidth(t)
     requires IsValidBid(s,op1.bid)
-    requires |s.mem[op1.bid]| == t
     requires op2.Int? && !op2.itype.signed
     ensures out.Ptr?
     ensures op1.offset + (op2.val * t) < |s.mem[op1.bid]| ==> IsValidPtr(s,out.bid,out.offset,t)
@@ -228,17 +193,39 @@ function evalGETELEMENTPTR(s:MemState,t:bitWidth,op1:Data,op2:Data): (out:Data)
     Ptr(op1.block,op1.bid,newOffset,t)
 }
 
-// function cpyBlock(b:Block, b':Block, i:int) : Block
-//     requires |b| > 0;
-//     requires |b| == |b'|
-//     requires 0 <= i && i < |b|
-//     ensures forall j :: (j < |b| && j>=i) ==> b[j] == b'[j];
-//     decreases i
-// {
-//     if i == 0 then b'
-//     else 
-//         var temp := b'[i := b[i]]; 
-//         cpyBlock(b,b',i-1)
-// }
+	
+function evalALLOCA(s:MemState, size:nat): (out:Data)
+    requires MemValid(s)
+    // requires Alloc(s,s',s.nextBlock,size);
+    requires validBitWidth(size);
+     ensures out.Ptr?;
+{
+    // && bid == s.nextBlock
+    // && s'.nextBlock == s.nextBlock + 1
+    // && s'.mem == s.mem[s.nextBlock := UninitBlock(size)]
+    var bid := s.nextBlock;
+    // assert Alloc(s,s',bid,size);
+    var d := (Ptr(bid,bid,0,size));
+    d
+}
+function AllocaStep(s:MemState, size:nat): (out:MemState)
+    requires MemValid(s);
+    ensures forall b :: b in s.mem ==> b in out.mem;
+    ensures forall bid:nat, offset:nat, size:bitWidth :: IsValidPtr(s,bid,offset,size) ==> IsValidPtr(out,bid,offset,size);
+    ensures Alloc(s,out,s.nextBlock,size);
+    ensures BlockValid(out.mem[s.nextBlock]);
+    ensures MemValid(out);
+{
+    // s'.nextBlock := s.nextBlock + 1;
+     var x := s.mem[s.nextBlock := UninitBlock(size)];
+     var y:MemState := MemState(x,s.nextBlock + 1);
+     assert forall b :: b in s.mem ==> b in y.mem;
+     assert forall bid:nat, offset:nat, size:bitWidth :: IsValidPtr(s,bid,offset,size) ==> IsValidPtr(y,bid,offset,size);
+     assert Alloc(s,y,s.nextBlock,size);
+     assert BlockValid(y.mem[s.nextBlock]);
+     assert MemValid(y);
+     y
+}
+
 
 }
