Dafny/examples/Challenge5/Challenge5Simple.i.dfy
@@ -1,0 +1,172 @@
+include "../../LLVM/llvm.i.dfy"
+include "../../LLVM/control_flow.i.dfy"
+include "../../LLVM/generalInstructionsBehavior.i.dfy"
+include "../../LLVM/types.dfy"
+include "../../LLVM/memory.i.dfy"
+include "../../LLVM/Operations/otherOperations.i.dfy"
+include "../../AbstractNonInterferenceProof.s.dfy"
+include "./Challenge5Code.s.dfy"
+include "./Challenge5_HelperLemmas.i.dfy"
+
+module challenge5 refines UpdatedAbstractNonInterferenceProof{ 
+    import opened challenge5Code
+    import opened challenge5_helpful_lemmas
+    import opened general_instructions_behaviors
+    import opened types
+    import opened memory
+    import opened other_operations_i
+
+
+   predicate stateFramingMultiValue(s:state,s':state)
+    {
+
+        challengeStateAssumptions(s);
+        var cipherText :| ValidOperand(s,cipherText);
+        var bytes_written :| ValidOperand(s,bytes_written);
+        var ops := {OperandContents(s,cipherText),OperandContents(s,bytes_written)};
+
+
+        ValidState(s)
+        && ValidState(s')
+        && forall op :: op in ops ==> 
+            (&& ValidData(s,op)
+            && ValidData(s',op)
+            && s.ok == s'.ok
+            && (forall lv :: (lv in s.lvs && !(s.lvs[lv] in ops)) ==> (lv in s'.lvs && s.lvs[lv] == s'.lvs[lv]))//(lv in s'.lv && s.lv[op] == s'.lv[op])
+            && (forall gv :: (gv in s.gvs && !(s.gvs[gv] in ops)) ==> (gv in s'.gvs && s.gvs[gv] == s'.gvs[gv]))
+            && (forall o:operand :: (o.D? && ValidOperand(s,o) && ValidOperand(s',o) && !(OperandContents(s,o) in ops) ) ==> (OperandContents(s,o) == OperandContents(s',o)))
+            && s.m == s'.m)
+    }
+
+
+    predicate RemovedBehaviors(b:behavior)
+    {
+        exists i,j :: 
+            (&& i >= 0 
+             && i <= |b|-2 
+             && j > i
+             && j < |b|
+             && evalBlock(encryptEmpty(),b[i],b[j])) 
+             && !stateFramingMultiValue(b[i],b[j])
+    }
+
+     
+    predicate preConds(codes:lvm_codes, s:lvm_state, s':lvm_state){
+        
+        && lvm_require(codes,challenge_prob_5_code_write_encrypted_simple(),s,s')
+        && codes.lvm_Codes?
+        && codes.tl.CNil?
+        && ValidState(s)
+        && challengeStateAssumptionsPred(s)
+    }
+
+    lemma challengeProb5PatchBehavior(codes:lvm_codes, s:lvm_state,s':lvm_state) 
+        returns (postB:behavior)
+
+        requires preConds(codes,s,s');
+
+        ensures ValidBehavior(postB);
+        ensures !MiniSpec(postBehavior(postB));
+        ensures !MiniSpec(preBehavior(postB));
+
+    {
+
+        postB := [s];
+        
+        var fullCode := challenge_prob_5_code_write_encrypted_simple();
+        var s' :|  lvm_require(codes, fullCode, s, s');
+        
+        assert s.ok;
+        assert codes.hd.Block?;
+        assert evalBlock(codes, s, s');
+        var r:state :| evalCode(codes.hd, s, r) && evalBlock(codes.tl, r, s') ;
+        var tail := codes.tl;
+ 
+        var codeBlock:lvm_codes := lvm_get_block(codes.hd);
+        var call := D(Ptr(0,0,0,1));
+
+        var bytes_written :| ValidOperand(s,bytes_written) && ValidState(s) && bytes_written.D? && D(Ptr(0,0,0,1)) == bytes_written;
+        assert codeBlock.hd == Ins(CALL(call,malloc(Int(0,IntType(8,false)))));
+        assert codeBlock.tl.lvm_Codes?;
+
+
+        var updatedB:behavior, unwrapedCode:lvm_codes, nextState:state := malloc_(postB, codeBlock, call, Int(0,IntType(8,false)), s');
+        assert updatedB[0] == s;
+
+        // assert AllocaStep(s.m,4) == nextState.m;
+        assert StateNext(s,nextState);
+        assert unwrapedCode == codeBlock.tl;
+        assert nextState == bls(updatedB);
+        var currState := nextState;
+
+        var mblock := D(Ptr(0,0,0,1));
+        assert unwrapedCode.hd == Ins(LLVM_MEMCPY(call,mblock,1,false));
+        assert ValidBehavior(updatedB); 
+        assert |updatedB| == 2;
+
+        updatedB, unwrapedCode, nextState := lvm_lemma_MemCpy(updatedB, unwrapedCode, r, call, mblock,1);
+
+         var call1 := D(Ptr(0,0,0,1));
+        assert StateNext(currState,nextState);
+        currState := nextState;
+        assert unwrapedCode.hd == Ins(CALL(call1,malloc(call1.d)));
+        assert ValidBehavior(updatedB); 
+        assert |updatedB| == 3;
+
+        updatedB, unwrapedCode, nextState := malloc_(updatedB, unwrapedCode, call1, Int(0,IntType(8,false)), s');
+        var IV_SIZE := D(Int(16,IntType(4,false)));
+        var KEY := D(Int(16,IntType(4,false)));
+        var cipherText := D(Ptr(0,0,0,1));
+        var call2 := D(Int(0,IntType(1,false)));
+
+       assert unwrapedCode.hd == Ins(CALL(call2,encrypt1(call,4,KEY,IV_SIZE,cipherText)));
+
+        currState := nextState;
+        assert ValidBehavior(updatedB); 
+        assert |updatedB| == 4;
+
+        updatedB, unwrapedCode, nextState := encrypt1_(updatedB, unwrapedCode, call2,call,4,KEY,IV_SIZE,cipherText, s');
+
+        assert unwrapedCode.hd == Ins(STORE(call2,bytes_written));
+        assert ValidBehavior(updatedB); 
+        assert |updatedB| == 5;
+
+        updatedB, unwrapedCode, nextState := lvm_lemma_Store(updatedB, unwrapedCode, r, call2, bytes_written);
+        assert ValidBehavior(updatedB); 
+        assert |updatedB| == 6;
+        
+        var call3 := D(Int(1,IntType(4,false)));
+        assert unwrapedCode.hd == Ins(CALL(call3,fwrite(bytes_written,4,1,D(Ptr(0,0,0,1)))));
+        
+        updatedB, unwrapedCode, nextState := fwrite_(updatedB, unwrapedCode, call3, bytes_written,4,1,D(Ptr(0,0,0,1)),s');
+        assert ValidBehavior(updatedB); 
+        assert |updatedB| == 7;
+        var cmp := D(Int(0,IntType(1,false)));
+
+        assert unwrapedCode.hd == Ins(ICMP(cmp,eq,4,call3,D(Int(0,IntType(4,false)))));
+        updatedB, unwrapedCode, nextState := lvm_lemma_Icmp(updatedB, unwrapedCode, s', cmp, eq,4,call3,D(Int(0,IntType(4,false))));
+        assert ValidBehavior(updatedB); 
+        assert |updatedB| == 8;
+        //
+        assert nextState == s';
+        assert unwrapedCode == lvm_CNil(); 
+        assert updatedB[0] == s;
+        assert updatedB[|updatedB|-1] == s';
+        assert BehaviorEvalsCode(codes.hd,updatedB);
+        assert !RemovedBehaviors(updatedB);
+        
+        postB := updatedB;
+    }
+
+
+    // predicate TestRemovedBehaviors(b:behavior)
+    // {
+    //     forall i,j :: 
+    //         (&& i >= 0 
+    //          && i <= |b|-2 
+    //          && j > i
+    //          && j < |b|
+    //          && evalBlock(encryptEmpty(),b[i],b[j])) 
+    //          ==> stateFramingMultiValue(b[i],b[j])
+    // }
+}
